committing changes to the 'tagging' pass

Tagging/Memory.v
@@ -6,9 +6,8 @@ From mathcomp Require Import ssreflect ssrfun ssrbool ssrnat seq eqtype.
 Require Import Common.Memory.
 Require Import Tags.
 
-
 Module Memory. (* : AbstractComponentMemory.*)
-  Definition block := list (value * mem_tag).
+  Definition block := list (tvalue * mem_tag).
 
   Implicit Types (b : Block.id).
 
@@ -22,11 +21,21 @@ Module Memory. (* : AbstractComponentMemory.*)
 
   Definition prealloc (bufs: {fmap Block.id -> (Component.id * (nat + list value))}) : t :=
     let init_block x := match x with
-                        | (c,inl size) => repeat (Undef,(MTag Other c)) size
+                        | (c,inl size) => repeat (tUndef, c) size
                         | (c,inr chunk) => to_tagged_block c chunk
                         end in
     {| content := mapm init_block bufs;
        nextblock := S (fold_left Nat.max (domm bufs) 0) |}.
+
+
+  Definition prealloc_c C (bufs: {fmap Block.id -> ((nat + list value))}) : t :=
+    let init_block x := match x with
+                        | inl size => repeat (tUndef, C) size
+                        | inr chunk => to_tagged_block C chunk
+                        end in
+    {| content := mapm init_block bufs;
+       nextblock := S (fold_left Nat.max (domm bufs) 0) |}.
+
 
   Definition empty :=
     {| content := emptym; nextblock := 0 |}.
@@ -37,12 +46,14 @@ Module Memory. (* : AbstractComponentMemory.*)
 
   Definition alloc (c : Component.id) m (size : nat) : mem * Block.id :=
     let fresh_block := nextblock m in
-    let chunk := repeat (Undef,(MTag Other c)) size in
+    let chunk := repeat (tUndef,c) size in
     ({| content := setm (content m) fresh_block chunk;
         nextblock := (1 + nextblock m) |},
      fresh_block).
 
-  Definition load m b i : option (value * mem_tag) :=
+
+
+  Definition load_b m b i : option (tvalue * mem_tag) :=
     match getm (content m) b with
     | Some chunk =>
       if (0 <=? i)%Z then nth_error chunk (Z.to_nat i)
@@ -50,7 +61,9 @@ Module Memory. (* : AbstractComponentMemory.*)
     | None => None
     end.
 
-  Definition store m b i v : option mem :=
+  Definition load m ptr : option (tvalue * mem_tag) := load_b m (Pointer.block ptr) (Pointer.offset ptr).
+
+  Definition store_b m b i v : option mem :=
     match getm (content m) b with
     | Some chunk =>
       if (0 <=? i)%Z then
@@ -63,6 +76,8 @@ Module Memory. (* : AbstractComponentMemory.*)
       else None
     | None => None
     end.
+
+  Definition store m ptr v : option mem := store_b m (Pointer.block ptr) (Pointer.offset ptr) v.
 
   Definition domm (m : t) := @domm nat_ordType block (content m).
 
