Tagging/Tags.v
@@ -13,6 +13,9 @@ From extructures Require Import fmap.
 Set Implicit Arguments.
 
 
+Section Tags.
+
+
 (* Value tags and tags for code *)
 
 
@@ -23,35 +26,150 @@ Definition code_tag : Type := option (Procedure.id * seq Component.id).
 
 (* Tag of Memory cell *)
 
-Record mem_tag : Type := MTag
+(* Record mem_tag : Type := MTag
   { vtag : value_tag;
-    color : Component.id }.
+    color : Component.id }.*)
 
-Definition def_mem_tag c := MTag Other c.
+Definition mem_tag := Component.id.
 
-  Definition to_tagged_cell (c : Component.id) (v : value) : value * mem_tag := (v,def_mem_tag c).
+Definition def_mem_tag c : mem_tag := c.
 
-  Definition to_tagged_block (c : Component.id) (l : list value) : list (value * mem_tag) := 
-    map (to_tagged_cell c) l.
+End Tags.
+
 
 
 (* PC tag *)
+Section PC.
 
 Inductive pc_tag : Type := Level : nat -> pc_tag.
 
 Definition level (pct : pc_tag) : nat := match pct with Level n => n end.
 
-Definition inc_pc_tag (pct : pc_tag) : pc_tag := Level (level pct + 1).
+Definition inc_pc_tag (pct : pc_tag) : pc_tag := Level (S (level pct)).
 
-(* Here: rather do an option thing? *)
-Definition dec_pc_tag (pct : pc_tag) : pc_tag := Level (level pct - 1).
+Definition dec_pc_tag (pct : pc_tag) : option pc_tag := match (level pct) with
+ | 0 => None
+ | S n => Some (Level n)
+end.
+
+Definition check_dec_pc_tag (pct : pc_tag) m : option pc_tag := match (level pct) with
+ | 0 => None
+ | S n => if Nat.eqb (S n) m then Some (Level n) else None
+end.
+
+Definition inc_ret (pct : pc_tag) := Ret (S (level pct)).
 
 
+End PC.
 
+Module Pointer.
+  Definition t : Type := Block.id * Block.offset.
+
+  Definition block (p : t) : Block.id :=
+    let '(b, _) := p in b.
+
+  Definition offset (p : t) : Block.offset :=
+    let '(_, o) := p in o.
+
+  Definition eq (p1 p2 : t) : bool :=
+    let '( b1, o1) := p1 in
+    let '( b2, o2) := p2 in
+    (Nat.eqb b1 b2) && (Z.eqb o1 o2).
+
+  Definition leq (p1 p2 : t) : option bool :=
+    let '( b1, o1) := p1 in
+    let '(b2, o2) := p2 in
+    if (Nat.eqb b1 b2) then
+      Some ((o1 <=? o2) % Z)
+    else
+      None.
+
+  Definition add (ptr : t) (offset : Z) : t :=
+    let '(b, o) := ptr in (b, (o+offset)%Z).
+
+  Definition sub (ptr : t) (offset : Z) : t :=
+    let '(b, o) := ptr in (b, (o-offset)%Z).
+
+  Definition inc (ptr : t) : t := add ptr 1.
+
+
+  Lemma add_preserves_block:
+    forall p n, block (add p n) = block p.
+  Proof.
+    intros p n.
+    destruct p as [b o].
+    reflexivity.
+  Qed.
+  Lemma inc_preserves_block:
+    forall p, block (inc p) = block p.
+  Proof.
+    intros p.
+    destruct p as [b o].
+    reflexivity.
+  Qed.
+
+  Lemma compose :
+    forall ptr,
+      (block ptr, offset ptr) = ptr.
+  Proof.
+    now intros [b o].
+  Qed.
+End Pointer.
+
+
+Section Values.
+
+
+  Inductive value : Type :=
+  | Int : Z -> value
+  | Ptr : Pointer.t -> value
+  | Undef : value.
+
+  Record tvalue := MVal
+   { vtag : value_tag;
+     val : value }.
+
+  Definition to_tvalue (v : value) : tvalue := MVal Other v.
+
+  Definition tUndef := to_tvalue Undef.
+
+  Definition to_tagged_cell (c : Component.id) (v : value) : tvalue * mem_tag := (to_tvalue v,def_mem_tag c).
+
+  Definition to_tagged_block (c : Component.id) (l : list value) : list (tvalue * mem_tag) := 
+    map (to_tagged_cell c) l.
+
+Definition eval_binop (op : binop) (v1 v2 : value) : value :=
+  match op, v1, v2 with
+  (* natural numbers *)
+  | Add,   Int n1, Int n2 => Int (n1 + n2)
+  | Minus, Int n1, Int n2 => Int (n1 - n2)
+  | Mul,   Int n1, Int n2 => Int (n1 * n2)
+  | Eq,    Int n1, Int n2 => Int (Util.Z.of_bool (n1  =? n2)%Z)
+  | Leq,   Int n1, Int n2 => Int (Util.Z.of_bool (n1 <=? n2)%Z)
+  (* pointer arithmetic *)
+  | Add,   Ptr p,  Int n  => Ptr (Pointer.add p n)
+  | Add,   Int n,  Ptr p  => Ptr (Pointer.add p n)
+  | Minus, Ptr p1, Ptr p2 => let '(b1, o1) := p1 in
+                             let '(b2, o2) := p2 in
+                             if (Nat.eqb b1 b2) then
+                               Int (o1 - o2)
+                             else
+                               Undef
+  | Minus, Ptr p,  Int n  => Ptr (Pointer.sub p n)
+  | Eq,    Ptr p1, Ptr p2 => Int (Util.Z.of_bool (Pointer.eq p1 p2))
+  | Leq,   Ptr p1, Ptr p2 => match Pointer.leq p1 p2 with
+                             | Some res => Int (Util.Z.of_bool res)
+                             | None     => Undef
+                             end
+  (* undefined operations *)
+  | _,     _,       _       => Undef
+  end.
+
+End Values.
 
 
 Module Register.
-  Definition t : Type := NMap (value * value_tag).
+  Definition t : Type := NMap tvalue.
 
   Definition to_nat (r : register) : nat :=
     match r with
@@ -64,43 +182,49 @@ Module Register.
     | R_ARG  => 6
     end.
 
-  Definition init :=
-    mkfmap [(to_nat R_ONE, (Undef,Other));
-            (to_nat R_COM, (Undef,Other));
-            (to_nat R_AUX1, (Undef,Other));
-            (to_nat R_AUX2, (Undef,Other));
-            (to_nat R_RA, (Undef,Other));
-            (to_nat R_SP, (Undef,Other));
-            (to_nat R_ARG, (Undef,Other))].
 
-  Definition get (r : register) (regs : t) : (value * value_tag) :=
+
+
+  Definition init :=
+    mkfmap [(to_nat R_ONE, tUndef);
+            (to_nat R_COM, tUndef);
+            (to_nat R_AUX1, tUndef);
+            (to_nat R_AUX2, tUndef);
+            (to_nat R_RA, tUndef);
+            (to_nat R_SP, tUndef);
+            (to_nat R_ARG, tUndef)].
+
+  Definition get (r : register) (regs : t) : tvalue :=
     match getm regs (to_nat r) with
     | Some v => v
     (* this should never happen (i.e. regs should be well-formed) *)
-    | None => (Undef,Other)
+    | None => tUndef
     end.
 
   Definition get_value (r : register) (regs : t) : value :=
     match getm regs (to_nat r) with
-    | Some (v,_) => v
+    | Some tv => val tv
     (* this should never happen (i.e. regs should be well-formed) *)
     | None => Undef
     end.
 
   Definition get_tag (r : register) (regs : t) : option value_tag :=
     match getm regs (to_nat r) with
-    | Some (_,vt) => Some vt
+    | Some tv => Some (vtag tv)
     (* this should never happen (i.e. regs should be well-formed) *)
     | None => None
     end.
 
   Definition set (r : register) (val : value) (vt : value_tag) (regs : t) : t :=
-    setm regs (to_nat r) (val,vt).
+    setm regs (to_nat r) (MVal vt val).
+
+  Definition tset (r : register) (tval : tvalue) (regs : t) : t :=
+    setm regs (to_nat r) tval.
 
 Definition invalidate regs := 
-[fmap (Register.to_nat R_ONE, (Undef,Other));(Register.to_nat R_COM, Register.get R_COM regs);
-      (Register.to_nat R_AUX1, (Undef,Other));(Register.to_nat R_AUX2, (Undef,Other));(Register.to_nat R_RA, Register.get R_RA regs);
-      (Register.to_nat R_SP, (Undef,Other));(Register.to_nat R_ARG, (Undef,Other))].
+[fmap (Register.to_nat R_ONE, tUndef);(Register.to_nat R_COM, Register.get R_COM regs);
+      (Register.to_nat R_AUX1, tUndef);(Register.to_nat R_AUX2, tUndef);(Register.to_nat R_RA, Register.get R_RA regs);
+      (Register.to_nat R_SP, tUndef);(Register.to_nat R_ARG, tUndef)].
 
   Lemma invalidate_eq : forall regs1 regs2,
     get R_COM regs1 = get R_COM regs2 ->
