Tagging/Language.v
@@ -1,0 +1,558 @@
+Require Import CompCert.Events.
+Require Import CompCert.Smallstep.
+Require Import CompCert.Behaviors.
+Require Import Common.Definitions.
+Require Import Common.Memory.
+Require Import Common.Traces.
+(* TL TODO: Ariths Export is a pain *)
+Require Import I2MP.Tmp.
+
+From mathcomp Require Import ssreflect ssrfun eqtype seq.
+From extructures Require Import fmap fset.
+
+Require Import Intermediate.Machine.
+(* Require Import Intermediate.GlobalEnv.
+Require Import MicroPolicies.LRC.
+Require Import Tmp.
+Require Import Linearize. *)
+Require Import Tags.
+Import Tags.Register.
+Require Import Tagging.Memory.
+Import Tagging.Memory.Memory.
+
+Require Import Lib.Extra.
+Require Import Lib.Monads.
+Import MonadNotations.
+Open Scope monad_scope.
+(* Import Intermediate.
+
+Require Import Source.Language. *)
+
+Definition proc_label : Set := Component.id * Procedure.id.
+
+Definition plabel : Set := label * option proc_label.
+
+Definition label_of (pl : plabel) : label := let (n,_) := pl in n.
+
+Variant instr :=
+| TrNop : instr
+| TrLabel : plabel -> instr
+(* register operations *)
+| TrConst : value -> register -> instr
+| TrMov : register -> register -> instr
+| TrBinOp : binop -> register -> register -> register -> instr
+(* memory operations *)
+| TrLoad : register -> register -> instr
+| TrStore : register -> register -> instr
+| TrAlloc : register -> register -> instr
+(* conditional and unconditional jumps *)
+| TrBnz : register -> label -> instr
+| TrJump : register -> instr
+| TrJalNat : label -> instr
+| TrJalProc : proc_label -> instr
+(* termination *)
+| TrHalt : instr.
+
+Definition code := NMap (seq (instr * code_tag)).
+
+
+
+(* 
+Definition executing (cde : code) (pc : Pointer.t) (i : instr) (tg : code_tag) (c : Component.id)  : Prop := 
+    exists C_code,
+    Pointer.component pc = c /\
+    cde c = Some C_code /\
+    (Pointer.offset pc >= 0) % Z /\
+    nth_error C_code (Z.to_nat (Pointer.offset pc)) = Some (i,tg). *)
+
+
+Fixpoint check_comp_belongs (c : Component.id) (l : seq Component.id) : Prop := match l with 
+ | nil => False
+ | c' :: l' => c = c' \/ check_comp_belongs c l'
+end.
+
+Fixpoint check_comp_belongs_b (c : Component.id) (l : seq Component.id) : bool := match l with 
+ | nil => false
+ | c' :: l' => if Nat.eqb c c' then true else check_comp_belongs_b c l'
+end.
+
+
+(* Stackless state *)
+
+Notation BigPointer := Common.Values.Pointer.t.
+
+Definition stackless : Type := Memory.t * Register.t * Pointer.t * pc_tag.
+
+Fixpoint find_label (cd : seq (instr * code_tag)) (l : label) : option Z :=
+  let fix aux c o :=
+      match c with
+      | [] => None
+      | (TrLabel l',_) :: c' =>
+        if Nat.eqb l (label_of l') then
+          Some o
+        else
+          aux c' (1 + o)%Z
+      | _ :: c' =>
+        aux c' (1 + o)%Z
+      end
+  in aux cd 0%Z.
+
+
+
+Definition find_label_in_comp (cde : code) (c : Component.id) (l : label) : option Pointer.t :=
+  match cde c with
+  | Some C_comp =>
+      match find_label C_comp l with
+      | Some offset => Some (c, offset)
+      | None => None
+      end
+  | None => None
+end.
+
+Fixpoint find_label_in_code_helper
+         (cde : code) (comps: list (Component.id * (seq (instr * code_tag))))
+         (l: label) : option Pointer.t :=
+  match comps with
+   | [] => None
+   | (comp_id,comp_code) :: comps' => match find_label_in_comp cde comp_id l with
+      | None => find_label_in_code_helper cde comps' l
+      | x => x
+    end
+  end.
+
+Definition find_label_in_code (cde : code) (l : label) : option Pointer.t :=
+  find_label_in_code_helper cde (elementsm cde) l.
+
+
+Fixpoint find_plabel (cd : seq (instr * code_tag)) (c : Component.id) (p : Procedure.id) : option Z :=
+  let fix aux cd o :=
+      match cd with
+      | [] => None
+      | (TrLabel (_,Some (c',p')),_) :: cd' =>
+        if Nat.eqb c c' && Nat.eqb p p' then
+          Some o
+        else
+          aux cd' (1 + o)%Z
+      | _ :: cd' =>
+        aux cd' (1 + o)%Z
+      end
+  in aux cd 0%Z.
+
+
+Definition find_plabel_in_code (cde : code) (c : Component.id) (p : Procedure.id) : option Pointer.t :=
+  match cde c with
+  | Some C_comp =>
+      match find_plabel C_comp c p with
+      | Some offset => Some (c, offset)
+      | None => None
+      end
+  | None => None
+end.
+
+
+
+(* 
+Inductive check_pc : code -> Pointer.t -> code_tag -> Prop :=
+| PcFall : forall cde pc tg i tni c, 
+    executing cde (Pointer.inc pc) i tni c ->
+    (* color tg = c -> *) check_pc cde pc tg.
+
+
+Inductive check_pc_jump : code -> mem_tag -> Pointer.t -> Component.id -> Prop :=
+ |PcJump : forall cde tg pc' i tni c c0,
+    executing cde (pc') i tni c ->
+    Pointer.component pc' = c0 -> check_pc_jump cde tg pc' c0.
+
+Inductive check_pc_call : Component.id -> code_tag -> Procedure.id -> Prop := 
+ | PcCall : forall c tni pid l, (* color ti = c ->  *)
+  tni = Some (pid,l) -> 
+  check_comp_belongs c l -> check_pc_call c tni pid.
+
+
+(* missing stuff *)
+Inductive check_pc_ret : Component.id -> code_tag -> Prop := 
+ | PcRet : forall c tni pid l, (* color ti = c ->  *)
+  tni = Some (pid,l) -> 
+  check_comp_belongs c l -> check_pc_ret c tni. *)
+
+
+(*** !IMPORTANT: PROTECT Return Adress registers with tags in a 'linear' way,
+                 so that they can't be copied ***)
+(* well-formedness & interfaces *)
+(* TODO Add Jal for (c,pid) type (TrJalProc), but intra compartment ?? 
+todo? (in order to reduce UB), allow TrJalNat to different components *)
+
+
+
+
+Open Scope monad_scope.
+(* remove locality of labels LATER *)
+
+Definition eval_step (cde: code) (s: stackless) : option (trace * stackless) :=
+  let '(mem, regs, pc, pct) := s in
+  (* fetch the next instruction to execute *)
+  if (Pointer.offset pc <? 0) % Z then
+    None
+  else
+      do C_code <- cde (Pointer.block pc);
+      do (instr,tag) <- nth_error C_code (Z.to_nat (Pointer.offset pc));
+    match instr with
+    | TrLabel _ =>
+      ret (E0, (mem, regs, Pointer.inc pc, pct))
+    | TrNop =>
+      ret (E0, (mem, regs, Pointer.inc pc, pct))
+    | TrConst v r =>
+      let regs' := Register.set r v Other regs in
+      ret (E0, (mem, regs', Pointer.inc pc, pct))
+    | TrMov r1 r2 => 
+      let tval := Register.get r1 regs in
+      let regs' := Register.tset r2 tval regs in
+      ret (E0, (mem, regs', Pointer.inc pc, pct))
+    | TrBinOp op r1 r2 r3 =>
+      let tv1 := Register.get r1 regs in
+      let tv2 := Register.get r2 regs in
+      let result := eval_binop op (val tv1) (val tv2) in
+      let regs' := Register.set r3 result Other regs in
+      (* Check to ensure that the value is not protected (return adress) *)
+      match (vtag tv1,vtag tv2) with
+        | (Other,Other) => ret (E0, (mem, regs', Pointer.inc pc, pct))
+        | (_,_) => None
+      end
+    | TrLoad r1 r2 => let tv := Register.get r1 regs in
+      match (val tv, vtag tv) with
+      | (Ptr ptr,Other) =>
+          do (v,c) <- Memory.load mem ptr;
+        if Component.eqb c (Pointer.block pc) then
+          match (vtag v) with
+            | Other =>
+              let regs' := Register.tset r2 v regs in
+              ret (E0, (mem, regs', Pointer.inc pc, pct))
+            | Ret n => 
+              let regs' := Register.tset r2 v regs in
+              do mem' <- Memory.store mem ptr (tUndef,Pointer.block pc);
+              ret (E0, (mem', regs', Pointer.inc pc, pct))
+          end
+        else
+          None
+      | _ => None
+      end
+    | TrStore r1 r2 => let tv := Register.get r1 regs in
+      match (val tv,vtag tv) with
+      | (Ptr ptr,Other) => 
+          if Component.eqb (Pointer.block ptr) (Pointer.block pc) then 
+            let tv2 := Register.get r2 regs in
+            match (vtag tv2) with
+            | Other =>
+              do mem' <- Memory.store mem ptr (Register.get r2 regs,Pointer.block pc);
+              ret (E0, (mem', regs, Pointer.inc pc, pct))
+            | Ret n => 
+              do mem' <- Memory.store mem ptr (Register.get r2 regs,Pointer.block pc);
+              let regs' := Register.tset r2 tUndef regs in
+              ret (E0, (mem', regs', Pointer.inc pc, pct))
+            end
+          else
+            None
+      | _ => None
+      end
+    | TrAlloc rptr rsize => let tv := Register.get rsize regs in
+      match (val tv, vtag tv) with
+      | (Int size,Other) =>
+        if (size <=? 0) % Z then
+          None
+        else
+          let (mem', block) := Memory.alloc (Pointer.block pc) mem (Z.to_nat size) in
+          let regs' := Register.set rptr (Ptr (block,0%Z)) Other regs in
+          ret (E0, (mem', regs', Pointer.inc pc, pct))
+      | _ => None
+      end
+    | TrBnz r l => let tv := Register.get r regs in
+      match (val tv, vtag tv) with
+      | (Int 0,Other) =>
+        ret (E0, (mem, regs, Pointer.inc pc, pct))
+      | (Int val,Other) =>
+        do pc' <- find_label_in_code cde l;
+        if Component.eqb (Pointer.block pc) (Pointer.block pc') then 
+          ret (E0, (mem, regs, pc', pct))
+        else
+          None
+      | _ => None
+      end
+    | TrJump r => let tv := Register.get r regs in
+      match (val tv, vtag tv) with
+      | (Ptr pc',Other) =>
+        if Component.eqb (Pointer.block pc') (Pointer.block pc) then
+          ret (E0, (mem, regs, pc', pct))
+        else
+          None
+      | (Ptr pc', Ret n) => 
+        do pctag' <- check_dec_pc_tag pct n;
+        if  (Component.eqb (Pointer.block pc') (Pointer.block pc)) then
+          None
+        else
+         if (Pointer.offset pc' <? 0) % Z then
+            None
+         else
+            do C_code' <- cde (Pointer.block pc');
+            do (ni,tni) <- nth_error C_code' (Z.to_nat (Pointer.offset pc'));
+            let tvcom := Register.get R_COM regs in
+            match (val tvcom,vtag tvcom) with
+            | (Int rcomval,Other) =>
+              let t := [ERet (Pointer.block pc) rcomval (Pointer.block pc')] in
+              ret (t, (mem, invalidate regs, pc', pctag'))
+            | _ => None
+            end
+      | _ => None
+      end
+    | TrJalNat l => 
+      do pc' <- find_label_in_comp cde (Pointer.block pc) l;
+      if Component.eqb (Pointer.block pc) (Pointer.block pc') then 
+        let regs' := Register.set R_RA (Ptr (Pointer.inc pc)) Other regs in
+        ret (E0, (mem, regs', pc', pct))
+      else
+        None
+    | TrJalProc (c',pid) =>
+      match find_plabel_in_code cde c' pid with 
+      | Some pc' => 
+       if (Pointer.offset pc' <? 0) % Z then
+         None
+       else
+       if negb (Component.eqb c' (Pointer.block pc')) then
+        None
+       else
+        if Component.eqb c' (Pointer.block pc) then
+          let regs' := Register.set R_RA (Ptr (Pointer.inc pc)) Other regs in
+          ret (E0, (mem, regs', pc', pct))
+        else 
+           do C_code' <- cde (Pointer.block pc');
+           do (ni,tni) <- nth_error C_code' (Z.to_nat (Pointer.offset pc'));
+           match tni with
+            | Some (pid',lc) => 
+              if Procedure.eqb pid pid' then 
+               if check_comp_belongs_b (Pointer.block pc) lc then
+                 let tvrcom := Register.get R_COM regs in
+                 match (val tvrcom,vtag tvrcom) with
+                 | (Int rcomval,Other) =>
+                     let regs' := Register.set R_RA (Ptr (Pointer.inc pc)) (inc_ret pct) regs in
+                     let t := [ECall (Pointer.block pc) pid rcomval (Pointer.block pc')] in
+                     ret (t, (mem, invalidate regs', pc', inc_pc_tag pct))
+                 | _ => None
+                 end
+               else None
+              else None
+             | _ => None
+            end
+       | None => None
+      end
+    | _ => None
+end.
+
+
+
+Fixpoint execN (n: nat) (cde: code) (st: stackless) : option Z + nat :=
+  match n with
+  | O => inr 3
+  | S n' =>
+    match eval_step cde st with
+    | None =>
+      let '(_, regs, _, _) := st in
+      let tvrcom := Register.get R_COM regs in
+      match (val tvrcom,vtag tvrcom) with
+      | (Int i,Other) => inl (Some i)
+      | (_,Other) => inr 4
+      | _ => inr 77
+      end
+    | Some (_, st') => execN n' cde st'
+    end
+  end.
+
+
+Record program : Type := mkProg {
+    prog_interface : Program.interface;
+    prog_code : code;
+    prog_buffers : {fmap Block.id -> Component.id * (nat + seq value)};
+    prog_main : bool }.
+
+
+(* Compile buffers *)
+
+Definition tag_buffers (pb : NMap {fmap Block.id -> nat + seq value}) : NMap {fmap Block.id -> Component.id * (nat + seq value)}:=
+ mapim (fun C f => mapim (fun b k => (C,k)) f) pb.
+
+Fixpoint clean_seq {T} (l : seq (option T)) : seq T := match l with
+ | [] => []
+ | None :: ls => clean_seq ls
+ | (Some x) :: ls => x :: clean_seq ls
+end.
+
+
+Definition fmap_rekeying {T : ordType} {T' : ordType} {S : Type} (f : {fmap T -> S}) (r : {fmap T -> T'}) : {fmap T' -> S} := 
+ let dom := clean_seq (map r (extructures.fmap.domm f)) in
+ let fn := fun x => match ((invm r) x) with None => None | Some y => f y end in
+mkfmapfp fn dom.
+
+Definition re_block_id C (pb : NMap {fmap Block.id -> nat + seq value}) (block_renum : {fmap (Component.id * Block.id) -> Block.id})  : option {fmap Block.id -> nat + seq value}:= 
+match pb C with
+ | None => None
+ | Some f => match ((currym block_renum) C) with None => None | Some g => Some (fmap_rekeying f g) end
+end.
+
+
+Fixpoint union_mem {T : ordType} {T' : ordType} {S : Type} l (f : T -> option {fmap T' -> S}) := match l with [] => emptym | x :: xs => 
+match (f x) with None => (union_mem xs f)
+ | Some y => unionm y (union_mem xs f) end
+end.
+
+Definition compile_buffs_renum (pb: NMap {fmap Block.id -> nat + seq value}) (block_renum : {fmap (Component.id * Block.id) -> Block.id}) :=
+union_mem (extructures.fmap.domm pb) (fun C => re_block_id C pb block_renum).
+
+
+Fixpoint add_key_aux {S} {T} (x : S) (l: seq T) : seq (S * T) := match l with [] => [] | y :: ys => (x,y) :: (add_key_aux x ys) end.
+
+Definition domm_to_seq {S} {T : ordType} {T' : ordType} (f : {fmap T' -> {fmap T -> S}}) (x : T') : seq T := match (f x) with None => [] | Some g => extructures.fmap.domm g end.
+
+Definition make_block_renum_fmap (pb: NMap {fmap Block.id -> nat + seq value}) (block_renum : Component.id -> Block.id -> Block.id) :=
+mkfmapf (fun x => match x with (C,b) => block_renum C b end) (foldr (fun C l => (add_key_aux C (domm_to_seq pb C)) ++ l) [] (extructures.fmap.domm pb)) .
+
+
+
+
+
+
+
+
+
+Definition max_block (m: NMap {fmap Block.id -> nat + seq value}) := let component_max_block map := foldl Nat.max 0 (extructures.fmap.domm map) in 
+ let max_block_ids := [seq component_max_block i | i <- codomm' m] in
+foldl Init.Nat.max 0 max_block_ids + 1.
+
+Definition fun_renum_block (m: NMap {fmap Block.id -> nat + seq value}) C b := C*(max_block m)+b.
+
+Definition compile_buffs (m: NMap {fmap Block.id -> nat + seq value}) := compile_buffs_renum m (make_block_renum_fmap m (fun_renum_block m)).
+
+
+
+
+(* Alloc initial memory *)
+
+
+
+Definition alloc_static_buffers p := prealloc (prog_buffers p).
+Definition prepare_initial_memory := alloc_static_buffers.
+
+
+(* temporarily removed
+Inductive step (cde : code) : stackless -> trace -> stackless -> Prop :=
+| Nop: forall st mem regs pc tg c pct,
+    executing cde pc TrNop tg c ->
+    check_pc cde pc tg ->
+    step cde (st, mem, regs, pc, pct) E0
+           (st, mem, regs, Pointer.inc pc, pct)
+
+| Label: forall st mem regs pc tg c pct l,
+    executing cde pc (TrLabel l) tg c ->
+    check_pc cde pc tg ->
+    step cde (st, mem, regs, pc, pct) E0
+           (st, mem, regs, Pointer.inc pc, pct)
+
+| Const: forall st mem regs regs' pc tg c pct r v,
+    executing cde pc (TrConst  v r) tg c ->
+    check_pc cde pc tg ->
+    Register.set r (imm_to_val v) regs = regs' ->
+    step cde (st, mem, regs, pc, pct) E0
+           (st, mem, regs', Pointer.inc pc, pct)
+
+| Mov: forall st mem regs regs' pc tg c pct r1 r2,
+    executing cde pc (TrMov r1 r2) tg c ->
+    check_pc cde pc tg ->
+    Register.set r2 (Register.get r1 regs) regs = regs' ->
+    step cde (st, mem, regs, pc, pct) E0
+           (st, mem, regs', Pointer.inc pc, pct)
+
+| BinOp: forall st mem regs regs' pc tg c pct r1 r2 r3 op,
+    executing cde pc (TrBinOp op r1 r2 r3) tg c ->
+    check_pc cde pc tg ->
+    let result := eval_binop op (Register.get r1 regs) (Register.get r2 regs) in
+    Register.set r3 result regs = regs' ->
+    step cde (st, mem, regs, pc, pct) E0
+           (st, mem, regs', Pointer.inc pc, pct)
+
+| Load: forall st mem regs regs' pc tg c pct r1 r2 ptr v,
+    executing cde pc (TrLoad r1 r2) tg c ->
+    check_pc cde pc tg ->
+    Register.get r1 regs = Ptr ptr ->
+    Pointer.component ptr = c ->
+    Memory.load mem ptr = Some v ->
+    Register.set r2 v regs = regs' ->
+    step cde (st, mem, regs, pc, pct) E0
+           (st, mem, regs', Pointer.inc pc, pct)
+
+| Store: forall st mem mem' regs pc tg c pct ptr r1 r2,
+    executing cde pc (TrStore r1 r2) tg c ->
+    check_pc cde pc tg ->
+    Register.get r1 regs = Ptr ptr ->
+    Pointer.component ptr =  c ->
+    Memory.store mem ptr (Register.get r2 regs) = Some mem' ->
+    step cde (st, mem, regs, pc, pct) E0
+           (st, mem', regs, Pointer.inc pc, pct)
+
+| Jal: forall st mem regs regs' pc tg c pct pc' l,
+    executing cde pc (TrJalNat l) tg c ->
+(*   check_pc cde pc tg ->*)
+(*    find_label_in_component G pc l = Some pc' -> *)
+    find_label_in_code cde l = Some pc' ->
+    Register.set R_RA (Ptr (Pointer.inc pc)) regs = regs' ->
+    check_pc_jump cde tg pc' c ->
+    step cde (st, mem, regs, pc, pct) E0
+           (st, mem, regs', pc', pct)
+
+| Jump: forall st mem regs pc tg c pct pc' r,
+    executing cde pc (TrJump r) tg c ->
+(*    check_pc cde pc tg ->*)
+    Register.get r regs = Ptr pc' ->
+(*    Pointer.component pc' = Pointer.component pc -> *)
+    check_pc_jump cde tg pc' c ->
+    step cde (st, mem, regs, pc, pct) E0
+           (st, mem, regs, pc', pct)
+
+| BnzNZ: forall st mem regs pc tg c pct pc' r l val,
+    executing cde pc (TrBnz r l) tg c ->
+(*    check_pc cde pc tg ->*)
+    Register.get r regs = Int val ->
+    (val <> 0) % Z ->
+    find_label_in_code cde l = Some pc' ->
+    check_pc_jump cde tg pc' c ->
+    step cde (st, mem, regs, pc, pct) E0
+           (st, mem, regs, pc', pct)
+
+| BnzZ: forall st mem regs pc tg c pct r l,
+    executing cde pc (TrBnz r l) tg c ->
+    check_pc cde pc tg ->
+    Register.get r regs = Int 0 ->
+    step cde (st, mem, regs, pc, pct) E0
+           (st, mem, regs, Pointer.inc pc, pct)
+
+| Alloc: forall st mem mem' regs regs' pc tg c pct rsize rptr size ptr,
+    executing cde pc (TrAlloc rptr rsize) tg c ->
+    check_pc cde pc tg ->
+    Register.get rsize regs = Int size ->
+    (size > 0) % Z ->
+    Memory.alloc mem c (Z.to_nat size) = Some (mem', ptr) ->
+    Register.set rptr (Ptr ptr) regs = regs' ->
+    step cde (st, mem, regs, pc, pct) E0
+           (st, mem', regs', Pointer.inc pc, pct)
+
+| Call: forall st mem regs regs' pc tg c pct pc' i tni c' pid call_arg,
+    executing cde pc (TrJalProc (c',pid)) tg c ->
+(*   check_pc cde pc tg ->*)
+(*    find_label_in_component G pc l = Some pc' -> *)
+    find_plabel_in_code cde c' pid = Some pc' ->
+    executing cde pc' i tni c' ->
+    c <> c' ->
+    check_pc_call c tni pid ->
+    Register.set R_RA (Ptr (Pointer.inc pc)) regs = regs' ->
+    Register.get R_COM regs = Int call_arg ->
+    step cde (st, mem, regs, pc, pct) [ECall c pid call_arg c']
+           (Pointer.inc pc :: st, mem, invalidate regs', pc', inc_pc_tag pct). *)
+
+
+
