Tagging/LinearizeCompartments.v
@@ -1,0 +1,146 @@
+Require Import CompCert.Events.
+Require Import CompCert.Smallstep.
+Require Import CompCert.Behaviors.
+Require Import Common.Definitions.
+Require Import Common.Memory.
+Require Import Common.Traces.
+(* TL TODO: Ariths Export is a pain *)
+
+From mathcomp Require Import ssreflect ssrfun eqtype seq.
+From extructures Require Import fmap fset.
+
+Require Import Intermediate.Machine.
+Require Import Intermediate.GlobalEnv.
+Require Import MicroPolicies.LRC.
+Require Import Tmp.
+Require Import Linearize.
+Require Import Tags.
+Require Import Tagging.Memory.
+Require Import Tagging.Language.
+
+Require Import Lib.Extra.
+Require Import Lib.Monads.
+Import MonadNotations.
+Open Scope monad_scope.
+
+
+Record compiler_env :=
+  { program : Intermediate.program ;
+    make_label : Component.id -> Procedure.id -> label ;
+    block_renum : Component.id -> Block.id -> Block.id ;
+  }.
+
+Definition ptr_to_ptr (ptr : BigPointer) (cenv : compiler_env) : Pointer.t := let '(c,b,o) := ptr in (block_renum cenv c b,o).
+
+Definition instr_to_transitional (cenv : compiler_env)
+           (c : Component.id) (i : Machine.instr) : instr :=
+  match i with
+  | ICall c' P => (TrJalProc (c',P)) 
+(* if beq_nat c c' then (TrJalProc (c',P)) (* ((TrJalNat (make_label cenv c' P)), def_mem_tag c) *)
+    else (TrJalProc (c',P)) *)
+  | IReturn => (TrJump R_RA)
+  | INop => TrNop
+  | ILabel l =>  TrLabel (l,None)
+  | IConst v r =>  
+    match v with 
+      | IInt z => TrConst (Int z) r
+      | IPtr ptr => TrConst (Ptr (ptr_to_ptr ptr cenv)) r
+    end
+  | IMov r r' => TrMov r r'
+  | IBinOp op r r' r'' => TrBinOp op r r' r''
+  | ILoad r r' => TrLoad r r'
+  | IStore r r' => TrStore r r'
+  | IAlloc r r' => TrAlloc r r'
+  | IBnz r l => TrBnz r l
+  | IJump r => TrJump r
+  | IJal l => TrJalNat l
+  | IHalt => TrHalt
+  end.
+
+
+Definition head_tag (cenv : compiler_env) (c : Component.id) (p : Procedure.id) : code_tag :=
+  let I := Intermediate.prog_interface (program cenv) in
+  let allowed_call_by (c' : Component.id) :=
+      Option.default false (do i <- getm I c ;
+                            do i' <- getm I c' ;
+                            Some ((p \in Component.export i) && ((c, p) \in Component.import i')))
+  in Some (p, filter allowed_call_by (domm I)).
+
+
+Definition linearize_proc (cenv : compiler_env)
+           (c : Component.id) (p : Procedure.id) : seq (instr * code_tag) :=
+  let code := Option.default [:: ] (do map <- getm (Intermediate.prog_procedures (program cenv)) c;
+                                    getm map p)
+  in ((TrLabel (make_label cenv c p, Some (c,p))), head_tag cenv c p) :: (map (fun x => (instr_to_transitional cenv c x,None)) code).
+
+Definition linearize_component (cenv : compiler_env) (c : Component.id) : seq (instr * code_tag) :=
+  let procs : seq Procedure.id :=
+      Option.default fset0 (do map <- getm (Intermediate.prog_procedures (program cenv)) c;
+                            Some (domm map)) in
+  flatten (map (linearize_proc cenv c) procs).
+
+
+Fixpoint compile_component_list {T} cenv (l : list (Component.id * T)) :=
+ match l with 
+  | [] => []
+  | (c,_) :: cs => (c,linearize_component cenv c) :: compile_component_list cenv cs
+end.
+
+Definition intermediate_to_transitional (cenv : compiler_env) : code := 
+mkfmap (compile_component_list cenv (elementsm (Intermediate.prog_procedures (program cenv)))).
+
+
+Definition max_component p := foldl Nat.max 0 (extructures.fmap.domm (Intermediate.prog_interface p)).
+
+Definition pre_linearize_code (p : Intermediate.program) : code :=
+  let lmax := max_label p in
+  let pmax := max_proc_id p in
+  let cmax := max_component p in
+  let cenv := {| program := p ;
+                 make_label := (fun c p => lmax + c * pmax + p + pmax * cmax +1) |} in 
+ intermediate_to_transitional cenv.
+
+(*  *)
+
+Print Intermediate.prepare_procedures_initial_memory_aux.
+
+Definition run_transitional cd fuel p :=
+    let '(mem, _, entrypoints) := Intermediate.prepare_procedures_initial_memory p in
+    let regs := Register.init in
+    match (find_plabel_in_code cd Component.main Procedure.main) with
+    | Some pc =>
+      execN fuel cd (mem,regs, pc, Level 0)
+    | None => inr 5
+end.
+
+Definition compile_run fuel (p : Intermediate.program) :=
+ run_transitional (pre_linearize p) fuel p.
+
+Close Scope monad_scope.
+
+
+Require Import Compiler.
+
+Definition compile_and_run_from_source := 
+fun (p : Source.program) (fuel : nat) =>
+match Compiler.compile_program p with
+| Some compiled_p => compile_run fuel compiled_p
+| None => inl None
+end.
+
+Require Export Extraction.Definitions.
+
+
+Definition compile_and_run_from_source_ex := 
+fun (p : Source.program) (fuel : nat) =>
+match Compiler.compile_program p with
+| Some compiled_p =>
+    match compile_run fuel compiled_p with
+    | inl (Some n) => print_ocaml_int (z2int n)
+    | inl None => print_error ocaml_int_1
+    | inr n => print_error (nat2int n)
+    end
+| None => print_error ocaml_int_0
+end.
+
+
